More moving

TransVal/smt.v
@@ -1,12 +1,23 @@
 Require Import List EqNat Bool.
-Require Import IL Exp Val  sexp bitvec.
+Require Import IL Exp Val bitvec.
 
 Set Implicit Arguments.
 
 (** Define what an argument list is **)
 Definition arglst := list exp.
 
-Definition vallst := list bitvec.
+Definition vallst := list val. (*bitvec.*)
+
+(**
+evalSexp evaluates an SMT expression given an environment that must! be total on
+every variable that may occur in a formula.
+**)
+
+Definition evalSexp E s : val(*bitvec*) :=
+match exp_eval E s with
+|Some v => v
+|None => default_val
+end.
 
 (** Define what uninterpreted function symbols are **)
 Definition pred := lab (*arglst -> bool*).
@@ -28,103 +39,6 @@ Inductive smt :Type :=
 Inductive pol:Type :=
 | source :pol
 | target :pol.
-
-(** Helper function to merge SMT options **)
-Definition combine (o1:option smt) (o2:option smt) :option smt :=
-match o1, o2 with
-| Some v1, Some v2 => Some (smtAnd v1 v2)
-| Some v1, _ => o1
-| _, _  => o2
-end.
-
-(** Function to generate the guard expression for one expression **)
-Fixpoint undef e :=
-match e with
-|BinOp n a b
- => match n with
-        | 0 =>  combine (undef a) (undef b)
-        | 1 =>  combine (undef a) (undef b)
-        | 2 =>  combine (undef a) (undef b)
-        | 3 =>  combine (undef a) (undef b)
-        | 4 =>  combine (undef a) (undef b)
-        | _ => match combine (undef a) (undef b) with
-                 | Some c => Some (smtAnd (smtNeg (constr b (Con (zext k (O::nil))))) c )
-                 | None =>  Some (smtNeg (constr b (Con (zext k (O::nil)))))
-               end
-    end
-|UnOp n a
- => undef a
-|Con v
- => None
-|Var v
- => None
-end.
-
-Fixpoint undefLift (el: list exp) :=
-match el with
-|nil => None
-| e::el' => combine (undef e) (undefLift el')
-end.
-
-(** Now the function that generates the guarding expressions for the smt translation function **)
-Fixpoint guard (p:pol) (e:exp) (cont:smt) :=
-match p, undef e with
-|source, Some g
- => smtAnd g cont
-|source, None
- => cont
-|target, Some g
- => smtImp g cont
-|target, None
- => cont
-end.
-
-Fixpoint guardList (p:pol) (l:arglst) (cont:smt) :=
-match l with
-| nil => cont
-| x:: l' => let c := guardList p l' cont in
-            match p, undef x with
-              | source, Some v =>  smtAnd v c
-              | target, Some v => smtImp v cont
-              | _, None => c
-            end
-end.
-
-Definition guardGen s p cont :=
-match s, p with
-| Some v, source => smtAnd v cont
-| Some v, target => smtImp v cont
-| None, _ => cont
-end.
-
-Fixpoint translateStmt (s:stmt) (p:pol) :smt :=
-match s, p with
-(*let x = e in s' *)
-| stmtExp x e s', _
-  =>  let smt' := translateStmt s' p in
-        let res := smtAnd (constr (Var x) e) smt'  in
-        guardGen (undef e) p res
-(* if e then s else t *)
-| stmtIf e s t, _
-  => let s' := translateStmt s p in
-        let t' := translateStmt t p in
-        let res := ite e s' t' in
-        guardGen (undef e) p res
-(* fun f x = t in s *)
-|  stmtLet x  t s, _ => smtFalse (* TODO *)
-(* extern ?? *)
-|  stmtExtern x f Y s, _ => smtFalse (* TODO *)
-(* f e, s*)
-| stmtGoto f e, source
-  =>  guardGen (undefLift e) p (funcApp f e)
-(* f e, t *)
-| stmtGoto f e, target
-  =>  guardGen (undefLift e) p ( smtNeg (funcApp f e ))
-| stmtReturn e, source
-  =>  guardGen (undef e) p (smtReturn e)
-| stmtReturn e, target
-  =>  guardGen  (undef e) p  ( smtNeg (smtReturn e))
-end.
 
 Fixpoint listGen (el:arglst) :=
 match el with
@@ -196,28 +110,6 @@ forall a b F E,
 Proof.
 intros.
 hnf. intros. eapply smtand_comm in H0. eapply H. assumption.
-Qed.
-
-Lemma combine_keep_undef:
-forall e1 e2,
-combine (undef e1) (undef e2) = None
--> undef e1 = None /\ undef e2 = None.
-
-Proof.
-intros.
-case_eq (undef e1); case_eq (undef e2); intros;
-rewrite H0 in H; rewrite H1 in H; try isabsurd; eauto.
-Qed.
-
-Lemma combine_keep_undef_list:
-forall e el,
-combine (undef e) (undefLift el) =  None
--> undef e = None /\ undefLift el = None.
-
-Proof.
-  intros.
-  case_eq (undef e); case_eq (undefLift el); intros;
-  rewrite H0 in H; rewrite H1 in H; try isabsurd; eauto.
 Qed.
 
   (*
