TransVal/Guards.v
@@ -1,0 +1,98 @@
+Require Import List EqNat Bool.
+Require Import IL Exp Val bitvec smt.
+
+(** Helper function to merge SMT options **)
+Definition combine (o1:option smt) (o2:option smt) :option smt :=
+match o1, o2 with
+| Some v1, Some v2 => Some (smtAnd v1 v2)
+| Some v1, _ => o1
+| _, _  => o2
+end.
+
+(** Function to generate the guard expression for one expression **)
+Fixpoint undef e :=
+match e with
+|BinOp n a b
+ => match n with
+        | 0 =>  combine (undef a) (undef b)
+        | 1 =>  combine (undef a) (undef b)
+        | 2 =>  combine (undef a) (undef b)
+        | 3 =>  combine (undef a) (undef b)
+        | 4 =>  combine (undef a) (undef b)
+        | _ => match combine (undef a) (undef b) with
+                 | Some c => Some (smtAnd (smtNeg (constr b (Con (zext k (O::nil))))) c )
+                 | None =>  Some (smtNeg (constr b (Con (zext k (O::nil)))))
+               end
+    end
+|UnOp n a
+ => undef a
+|Con v
+ => None
+|Var v
+ => None
+end.
+
+Fixpoint undefLift (el: list exp) :=
+match el with
+|nil => None
+| e::el' => combine (undef e) (undefLift el')
+end.
+
+(** Now the function that generates the guarding expressions for the smt translation function **)
+Fixpoint guard (p:pol) (e:exp) (cont:smt) :=
+match p, undef e with
+|source, Some g
+ => smtAnd g cont
+|source, None
+ => cont
+|target, Some g
+ => smtImp g cont
+|target, None
+ => cont
+end.
+
+Fixpoint guardList (p:pol) (l:arglst) (cont:smt) :=
+match l with
+| nil => cont
+| x:: l' => let c := guardList p l' cont in
+            match p, undef x with
+              | source, Some v =>  smtAnd v c
+              | target, Some v => smtImp v cont
+              | _, None => c
+            end
+end.
+
+Definition guardGen s p cont :=
+match s, p with
+| Some v, source => smtAnd v cont
+| Some v, target => smtImp v cont
+| None, _ => cont
+end.
+
+Lemma combine_keep_undef:
+forall e1 e2,
+combine (undef e1) (undef e2) = None
+-> undef e1 = None /\ undef e2 = None.
+
+Proof.
+intros.
+case_eq (undef e1); case_eq (undef e2); intros;
+rewrite H0 in H; rewrite H1 in H; try isabsurd; eauto.
+Qed.
+
+Lemma combine_keep_undef_list:
+forall e el,
+combine (undef e) (undefLift el) =  None
+-> undef e = None /\ undefLift el = None.
+
+Proof.
+  intros.
+  case_eq (undef e); case_eq (undefLift el); intros;
+  rewrite H0 in H; rewrite H1 in H; try isabsurd; eauto.
+Qed.
+
+  (*
+  *** Local Variables: ***
+  *** coq-load-path: (("../" "Lvc")) ***
+  *** End: ***
+  *)
