TransVal/ILFtoSMT.v
@@ -1,0 +1,36 @@
+Require Import smt Guards IL.
+
+Fixpoint translateStmt (s:stmt) (p:pol) :smt :=
+match s, p with
+(*let x = e in s' *)
+| stmtExp x e s', _
+  =>  let smt' := translateStmt s' p in
+        let res := smtAnd (constr (Var x) e) smt'  in
+        guardGen (undef e) p res
+(* if e then s else t *)
+| stmtIf e s t, _
+  => let s' := translateStmt s p in
+        let t' := translateStmt t p in
+        let res := ite e s' t' in
+        guardGen (undef e) p res
+(* fun f x = t in s *)
+|  stmtLet x  t s, _ => smtFalse (* TODO *)
+(* extern ?? *)
+|  stmtExtern x f Y s, _ => smtFalse (* TODO *)
+(* f e, s*)
+| stmtGoto f e, source
+  =>  guardGen (undefLift e) p (funcApp f e)
+(* f e, t *)
+| stmtGoto f e, target
+  =>  guardGen (undefLift e) p ( smtNeg (funcApp f e ))
+| stmtReturn e, source
+  =>  guardGen (undef e) p (smtReturn e)
+| stmtReturn e, target
+  =>  guardGen  (undef e) p  ( smtNeg (smtReturn e))
+end.
+
+  (*
+  *** Local Variables: ***
+  *** coq-load-path: (("../" "Lvc")) ***
+  *** End: ***
+  *)
