TransVal/transval.v
@@ -2,7 +2,7 @@ Require Import List Arith.
 Require Import IL Annotation AutoIndTac Bisim Exp MoreExp Coherence Fresh Util.
 Require Import SetOperations Sim Var.
 Require Import bitvec sexp smt nofun noGoto freeVars.
-Require Import Compute tvalTactics TUtil GuardProps ComputeProps.
+Require Import Compute Guards ILFtoSMT tvalTactics TUtil GuardProps ComputeProps.
 
 Definition smtCheck (s:stmt) (t:stmt) :=
 smtAnd (translateStmt s source) (translateStmt t target).
